WIP commit to show to supervisor

il1Script.sml
@@ -1,14 +1,17 @@
-open HolKernel boolLib bossLib wordsTheory wordsLib listTheory Parse IndDefLib finite_mapTheory relationTheory arithmeticTheory l1Theory;
+open HolKernel boolLib bossLib wordsTheory wordsLib listTheory Parse IndDefLib finite_mapTheory relationTheory arithmeticTheory l1Theory pred_setTheory;
 
 val _ = new_theory "il1";
 
 val _ = type_abbrev("loc", ``:num``);
 
-val _ = type_abbrev("int", ``:word16``);
+val _ = type_abbrev("int", ``:num``);
 
 val _ = type_abbrev("state", ``:loc |-> int``);
 
 val _ = type_abbrev("pred", ``:state -> bool``);
+
+val _ = Hol_datatype `il1_loc = User of loc
+                              | Compiler of loc`; 
 
 val _ = Hol_datatype `il1_value = IL1_ESkip
                                 | IL1_Integer of int
@@ -17,54 +20,14 @@ val _ = Hol_datatype `il1_value = IL1_ESkip
 val _ = Hol_datatype `il1_expr = IL1_Value of il1_value
                                | IL1_Plus of il1_expr => il1_expr
                                | IL1_Geq of il1_expr => il1_expr
-                               | IL1_Deref of loc
+                               | IL1_Deref of il1_loc
                                | IL1_EIf of il1_expr => il1_expr => il1_expr`;
 
 val _ = Hol_datatype `il1_stm = IL1_Expr of il1_expr
-                              | IL1_Assign of loc => il1_expr
+                              | IL1_Assign of il1_loc => il1_expr
                               | IL1_Seq of il1_stm => il1_stm
                               | IL1_SIf of il1_expr => il1_stm => il1_stm
                               | IL1_While of il1_expr => il1_stm`;
-
-val contains_expr_def = Define `
-    (contains_expr l (IL1_Value v) = F) /\
-    (contains_expr l (IL1_Plus e1 e2) = contains_expr l e1 \/ contains_expr l e2) /\
-    (contains_expr l (IL1_Geq e1 e2) = contains_expr l e1 \/ contains_expr l e2) /\
-    (contains_expr l1 (IL1_Deref l2) = (l1 = l2)) /\
-    (contains_expr l (IL1_EIf e1 e2 e3) = contains_expr l e1 \/ contains_expr l e2 \/ contains_expr l e3)`;
-
-val contains_def = Define `
-    (contains l (IL1_Expr e) = contains_expr l e) /\
-    (contains l1 (IL1_Assign l2 e) = (l1 = l2) \/ contains_expr l1 e) /\
-    (contains l (IL1_Seq e1 e2) = contains l e1 \/ contains l e2) /\
-    (contains l (IL1_SIf e1 e2 e3) = contains_expr l e1 \/ contains l e2 \/ contains l e3) /\
-    (contains l (IL1_While e1 e2) = contains_expr l e1 \/ contains l e2)`;
-
-val max_loc_expr_def = Define `
-    (max_loc_expr (IL1_Value v) = 0) /\
-    (max_loc_expr (IL1_Plus e1 e2) = MAX (max_loc_expr e1) (max_loc_expr e2)) /\
-    (max_loc_expr (IL1_Geq e1 e2) = MAX (max_loc_expr e1) (max_loc_expr e2)) /\
-    (max_loc_expr (IL1_Deref l) = l) /\
-    (max_loc_expr (IL1_EIf e1 e2 e3) = MAX (MAX (max_loc_expr e1) (max_loc_expr e2)) (max_loc_expr e3))`;
-
-val max_loc_def = Define `
-    (max_loc (IL1_Expr e) = max_loc_expr e) /\
-    (max_loc (IL1_Assign l2 e) = MAX l2 (max_loc_expr e)) /\
-    (max_loc (IL1_Seq e1 e2) = MAX (max_loc e1) (max_loc e2)) /\
-    (max_loc (IL1_SIf e1 e2 e3) = MAX (MAX (max_loc_expr e1) (max_loc e2)) (max_loc e3)) /\
-    (max_loc (IL1_While e1 e2) = MAX (max_loc_expr e1) (max_loc e2))`;
-
-
-val UNUSED_UPPER_LOCS_EXPR_THM = store_thm(
-    "UNUSED_UPPER_LOCS_EXPR_THM",
-    ``!e n.max_loc_expr e < n ==> ~contains_expr n e``,
-    Induct_on `e` THEN EVAL_TAC THEN FULL_SIMP_TAC (srw_ss ()) [MAX_DEF]);
-
-val UNUSED_UPPER_LOCS_THM = store_thm(
-    "UNUSED_UPPER_LOCS_THM",
-    ``!e n.max_loc e < n==> ~contains n e``,
-    Induct_on `e` THEN EVAL_TAC
-    THEN FULL_SIMP_TAC (srw_ss ()) [MAX_DEF, UNUSED_UPPER_LOCS_EXPR_THM]);
 
 val (bs_il1_expr_rules, bs_il1_expr_induction, bs_il1_expr_ecases) = Hol_reln `
     (* Values *)
@@ -87,6 +50,10 @@ val (bs_il1_expr_rules, bs_il1_expr_induction, bs_il1_expr_ecases) = Hol_reln `
         l ∈ FDOM s
     ==> bs_il1_expr (IL1_Deref l, s) (IL1_Integer (s ' l))) /\
 
+    (!l s.
+        l ∉ FDOM s
+    ==> bs_il1_expr (IL1_Deref l, s) (IL1_Integer 0)) /\
+
     (* EIf *)
     (!e1 e2 e3 s v.
         (bs_il1_expr (e1, s) (IL1_Boolean T) /\
@@ -106,8 +73,7 @@ val (bs_il1_rules, bs_il1_induction, bs_il1_ecases) = Hol_reln `
 
     (* Assign *)
     (!l e s n.
-       (l ∈ FDOM s /\
-        bs_il1_expr (e, s) (IL1_Integer n))
+        bs_il1_expr (e, s) (IL1_Integer n)
     ==> bs_il1 (IL1_Assign l e, s) IL1_ESkip (s |+ (l, n))) /\
 
     (* Seq *)
@@ -142,12 +108,12 @@ val l1_to_il1_pair_def = Define `
     (l1_to_il1_pair lc (B_Value (B_N n)) = (IL1_Expr (IL1_Value IL1_ESkip), IL1_Value (IL1_Integer n), lc)) /\
     (l1_to_il1_pair lc (B_Value (B_B b)) = (IL1_Expr (IL1_Value IL1_ESkip), IL1_Value (IL1_Boolean b), lc)) /\
     (l1_to_il1_pair lc (B_Value B_Skip) = (IL1_Expr (IL1_Value IL1_ESkip), IL1_Value IL1_ESkip, lc)) /\
-    (l1_to_il1_pair lc (B_Deref l) = (IL1_Expr (IL1_Value IL1_ESkip), IL1_Deref l, lc)) /\
+    (l1_to_il1_pair lc (B_Deref l) = (IL1_Expr (IL1_Value IL1_ESkip), IL1_Deref (User l), lc)) /\
 
     (l1_to_il1_pair lc (B_Assign l e) =
         let (sl, e', lc2) = l1_to_il1_pair lc e
         in
-            (IL1_Seq sl (IL1_Assign l e'), IL1_Value IL1_ESkip,lc2)) /\
+            (IL1_Seq sl (IL1_Assign (User l) e'), IL1_Value IL1_ESkip,lc2)) /\
 
     (l1_to_il1_pair lc (B_Seq e1 e2) =
         let (sl1, e1', lc2) = l1_to_il1_pair lc e1 in
@@ -171,16 +137,39 @@ val l1_to_il1_pair_def = Define `
         let (sl1, e1', lc2) = l1_to_il1_pair lc e1 in
         let (sl2, e2', lc3) = l1_to_il1_pair lc2 e2
         in
-            (IL1_Seq (IL1_Seq sl1 (IL1_Assign (lc3 + 1) e1')) sl2, IL1_Plus (IL1_Deref (lc3 + 1)) e2', lc3 + 1)) /\ 
+            (IL1_Seq (IL1_Seq sl1 (IL1_Assign (Compiler lc3) e1')) sl2, IL1_Plus (IL1_Deref (Compiler lc3)) e2', lc3 + 1)) /\ 
 
     (l1_to_il1_pair lc (B_Geq e1 e2) =
         let (sl1, e1', lc2) = l1_to_il1_pair lc e1 in
         let (sl2, e2', lc3) = l1_to_il1_pair lc2 e2
         in
-            (IL1_Seq (IL1_Seq sl1 (IL1_Assign (lc3 + 1) e1')) sl2, IL1_Geq (IL1_Deref (lc3 + 1)) e2', lc3 + 1))
+            (IL1_Seq (IL1_Seq sl1 (IL1_Assign (Compiler lc3) e1')) sl2, IL1_Geq (IL1_Deref (Compiler lc3)) e2', lc3 + 1))
 `;
 
-val l1_to_il1_def = Define `l1_to_il1 e = let (s, te, lc) = l1_to_il1_pair (max_loc_l1 e) e in IL1_Seq s (IL1_Expr te)`;
+val l1_to_il1_def = Define `l1_to_il1 e = let (s, te, lc) = l1_to_il1_pair 0 e in IL1_Seq s (IL1_Expr te)`;
+
+val l1_il1_val_def = Define `(l1_il1_val (B_N n) = IL1_Integer n) /\
+(l1_il1_val (B_B b) = IL1_Boolean b) /\
+(l1_il1_val (B_Skip) = IL1_ESkip)`;
+
+val pair_first_def = Define `pair_first (a, b) = a`;
+val pair_second_def = Define `pair_second (a, b) = b`;
+
+val minimal_store_def = Define `minimal_store e s = !k.k ∈ FDOM s ==> contains_l1 k e`;
+
+val MAX_LOC_MIN_STORE_THM = store_thm("MAX_LOC_MIN_STORE_THM",
+``!e s.minimal_store e s ==> !k.k ∈ FDOM s ==> k <= max_loc_l1 e``,
+RW_TAC (srw_ss ()) [minimal_store_def] THEN
+`contains_l1 k e` by FULL_SIMP_TAC (srw_ss ()) [] THEN
+CCONTR_TAC THEN
+FULL_SIMP_TAC (srw_ss ()) [NOT_LESS_EQUAL, (fetch "l1" "UNUSED_UPPER_LOCS_THM")]);
+
+
+
+!p v s'.big_step p v s' ==> ?s1.(bs_il1 (l1_to_il1 (pair_first p), MAP_KEYS User (pair_second p)) (l1_il1_val v) s1)
+
+HO_MATCH_MP_TAC (fetch "l1" "big_step_strongind")
+THEN RW_TAC (srw_ss ()) [pair_first_def, pair_second_def, l1_il1_val_def]
 
 
 val _ = export_theory ();
